trying to implement adding two

VerifiedCompiler/Ast.lean
@@ -2,3 +2,4 @@ inductive Expr
 | Num (n : Nat)
 | Add1 (e : Expr)
 | Sub1 (e : Expr)
+| Add (e₁ : Expr) (e₂ : Expr)
