VerifiedCompiler/Compile.lean
@@ -10,3 +10,8 @@ def compile_expr : Expr → List Directive
   (compile_expr e) ++ [Sub (Reg Rax, Imm 1)]
 | Add1 e =>
   (compile_expr e) ++ [Add (Reg Rax, Imm 1)]
+| Expr.Add e₁ e₂ =>
+  compile_expr e₁
+  ++ [ Push (Reg Rax) ]
+  ++ compile_expr e₂
+  ++ [ Add (Reg Rax, Pop) ]
