VerifiedCompiler/Process.lean
@@ -5,26 +5,41 @@ open Directive Operand Register Expr
 
 structure ProcessorState where
   rax : Nat
+  rcx : Nat
+  stack : List Nat
 
 def ProcessorState.regVal (st : ProcessorState) : Register → Nat
 | Rax => st.rax
+| Rcx => st.rcx
 
 def ProcessorState.opVal (st : ProcessorState) : Operand → Nat
 | Imm i => i
 | Reg r => st.regVal r
+| Pop =>
+  match st.stack with
+  | [] => 0
+  | v :: _ => v
 
 def ProcessorState.setReg (st : ProcessorState) (val : Nat) : Register → ProcessorState
 | Rax => { st with rax := val }
+| Rcx => { st with rcx := val }
+
+def ProcessorState.stackPush (st : ProcessorState) (val : Nat) : ProcessorState
+  := { st with stack := val :: st.stack }
 
 def processDirective (st : ProcessorState) : Directive → ProcessorState
 | Mov (Reg r, o) => st.setReg (st.opVal o) r
 | Mov (Imm _, _) => st
+| Mov (Pop, _) => st
+| Push o => st.stackPush (st.opVal o)
 | Directive.Add (Reg r, o) => st.setReg (st.regVal r + st.opVal o) r
 | Directive.Add (Imm _, _) => st
+| Directive.Add (Pop, _) => st
 | Directive.Sub (Reg r, o) => st.setReg (st.regVal r - st.opVal o) r
 | Directive.Sub (Imm _, _) => st
+| Directive.Sub (Pop, _) => st
 
-def Processor.evalToState : List Directive → ProcessorState :=
-List.foldl processDirective {rax := 0}
+@[simp] def Processor.evalToState : List Directive → ProcessorState :=
+List.foldl processDirective {rax := 0, rcx := 0, stack := []}
 
-def Processor.eval (ds : List Directive) : Nat := (evalToState ds).rax
+@[simp] def Processor.eval (ds : List Directive) : Nat := (evalToState ds).rax
