VerifiedCompiler/Asm.lean
@@ -1,11 +1,14 @@
 inductive Register
 | Rax
+| Rcx
 
 inductive Operand
 | Reg (r : Register)
+| Pop
 | Imm (i : Nat)
 
 inductive Directive
 | Mov (st : Operand × Operand)
 | Add (st : Operand × Operand)
 | Sub (st : Operand × Operand)
+| Push (st : Operand)
