VerifiedCompiler/Compare.lean
@@ -4,11 +4,22 @@ import VerifiedCompiler.Interpret
 
 import VerifiedCompiler.LoVelib
 
-open Value Expr
+open Value Expr Directive Register Operand
 
-def Processor.evalToValue (ds : List Directive) : Value :=
+@[simp] def Processor.evalToValue (ds : List Directive) : Value :=
   Integer (Processor.eval ds)
 
+
+theorem moving
+    (prog : Expr) (st_nopush st_push : ProcessorState)
+    (eval_nopush : Processor.evalToState (compile_expr prog) = st_nopush)
+    (eval_push : Processor.evalToState (compile_expr prog ++ [Push (Reg Rax)]) = st_push)
+    : st_push = { st_nopush with stack := st_push.rax :: st_nopush.stack }
+    :=
+    by sorry
+
+
+#check List.foldl_append
 
 theorem correctness :
   ∀ prog : Expr, Processor.evalToValue (compile_expr prog) = interpret_expr prog
@@ -28,7 +39,7 @@ theorem correctness :
       | nil => simp
       | cons hd tl =>
         have hfold_concat :=
-          List.foldl_concat processDirective { rax := 0 }
+          List.foldl_concat processDirective { rax := 0, rcx := 0, stack := [] }
             (Directive.Sub (Operand.Reg Register.Rax, Operand.Imm 1)) (hd :: tl)
         rw [hfold_concat]
         rfl
@@ -43,7 +54,28 @@ theorem correctness :
       cases (compile_expr e) with
       | nil => simp
       | cons hd tl =>
-        have hfold_concat := List.foldl_concat processDirective { rax := 0 }
+        have hfold_concat := List.foldl_concat processDirective { rax := 0, rcx := 0, stack := [] }
             (Directive.Add (Operand.Reg Register.Rax, Operand.Imm 1)) (hd :: tl)
         rw [hfold_concat]
         rfl
+  | Expr.Add e₁ e₂ =>
+    by
+      have ih₁ := correctness e₁
+      have ih₂ := correctness e₂
+      simp [interpret_expr] at *
+      rw [←ih₁, ←ih₂]
+      simp
+      rw [compile_expr]
+
+      have smth := moving e₁ (Processor.evalToState (compile_expr e₁))
+                            (Processor.evalToState (compile_expr e₁ ++ [Push (Reg Rax)]))
+                            (by rfl) (by rfl)
+      simp only [Processor.evalToState] at smth
+      have llsee := List.foldl_append processDirective { rax := 0, rcx := 0, stack := [] } (compile_expr e₁ ++ [Push (Reg Rax)]) (compile_expr e₂ ++ [Add (Reg Rax, Pop)])
+      have heq : (compile_expr e₁ ++ [Push (Reg Rax)]) ++ (compile_expr e₂ ++ [Add (Reg Rax, Pop)])
+                = compile_expr e₁ ++ [Push (Reg Rax)] ++ compile_expr e₂ ++ [Add (Reg Rax, Pop)] := by simp
+      rw [heq] at llsee
+      rw [llsee]
+      rw [smth]
+
+      sorry
